Flapjack/Tests.lean
@@ -1,4 +1,5 @@
 import Flapjack.Test.Basics
+import Flapjack.Test.SourceSemantics
 import Flapjack.Test.Compile
 import Flapjack.Test.RiscVMemory
 import Flapjack.Test.RiscV
